Refactor tactics and common elements

src/named/Tactics.v
@@ -1,5 +1,5 @@
 (*********************************************
-A partial recognizer for well-formed languages
+Tactics for deriving well-formed languages
 **********************************************)
 
 
@@ -9,352 +9,145 @@ Unset Strict Implicit.
 Unset Printing Implicit Defensive.
 Set Bullet Behavior "Strict Subproofs".
 
-From Utils Require Import Utils.
-From Named Require Import Exp Rule Core.
 
 From Ltac2 Require Import Ltac2.
-Require Ltac2.List Ltac2.Option Ltac2.Std.
-(*TODO: copied from stdlib; need to update version?*)
-Ltac2 of_goal () := Fresh.Free.of_ids (List.map (fun (id, _, _) => id) (Control.hyps ())).
-
-Ltac2 in_goal id := Fresh.fresh (of_goal ()) id.
-
-Ltac2 fresh s := in_goal (Option.get (Ident.of_string s)).
-
-
-(* taken from https://github.com/coq/coq/issues/11641 *)
-Ltac2 my_change2 (a : constr) (b : constr) :=
-  ltac1:( a b |- change a with b ) (Ltac1.of_constr a) (Ltac1.of_constr b).
-
-
-Ltac2 all_red_flags :=
-  { Std.rBeta := true;
-  Std.rMatch := true;
-  Std.rFix := true;
-  Std.rCofix := true;
-  Std.rZeta := true;
-  Std.rDelta := true;
-  Std.rConst := []
-}.
-
-(*
-tests whether two terms are equal,
-unifying evars as necessary.
-EFFECT: adds a = b as a hypothesis if true,
-possibly instantiating evars in the process
- *)
-Ltac2 eequal a b :=
-  Control.plus
-    (fun () =>
-       let heq := fresh "Heq" in
-       assert ($a = $b)>[solve[f_equal; eauto]|]; true)
-    (fun _ => false).
-
-Ltac2 change_cbv e :=
-  my_change2 e (Std.eval_cbv all_red_flags e).
-
-(* Attempts to clear a goal of the form
-   'a \in l', unifying evars as necessary *)
-Ltac2 Type exn ::= [UnifyInFailure].
-Ltac2 rec unify_in () :=
-  lazy_match! goal with
-   | [|- is_true (?r \in ?r'::?l)] =>
-      change_cbv r;
-      rewrite in_cons;
-      ltac1:(apply /orP);
-      match eequal r r' with
-      | true => left;ltac1:(by apply /eqP)
-      | false => right; unify_in()
-      end
-   | [|- is_true (_ \in [::])] => Control.zero UnifyInFailure
-   | [|- is_true (_ \in ?l)] => change_cbv l; unify_in ()
-  end.
-
+From Utils Require Import Utils.
+From Named Require Import Exp ARule.
+From Named Require Import IExp IRule ICore.
 Require Import String.
-  (*
-Ltac2 try f :=
-  Control.enter
-    (fun () => Control.plus f (fun _ => ())).*)
+
+Require Import Named.Recognizers.
+Require Coq.derive.Derive.
+
+Set Default Proof Mode "Ltac2".
 
 
-Ltac2 goal_lang () :=
+(* TODO: move to tactics*)
+
+
+(* TODO: move*)
+Definition id_subst : list string -> Exp.subst :=
+  map (fun x => (x, Exp.var x)).
+
+Lemma id_subst_exp_identity e args : Exp.exp_subst (id_subst args) e = e.
+Admitted.
+Lemma id_subst_sort_identity t args : Exp.sort_subst (id_subst args) t = t.
+Admitted.
+
+Lemma id_subst_fold x args : (x,Exp.var x)::(id_subst args) = id_subst (x::args).
+Proof using.
+  simpl; reflexivity.
+Qed.
+
+Lemma sort_subst_fold s n l
+  : Exp.srt n (map (Exp.exp_subst s) l)
+    = Exp.apply_subst s (Exp.srt n l).
+Proof using .
+  simpl; reflexivity.
+Qed.
+
+Ltac2 solve_in () :=
+  solve [ cbv; reflexivity
+        | repeat (rewrite in_cons);
+          rewrite in_nil;
+          rewrite Bool.orb_false_r;
+          ltac1:(apply /eqP);
+          reflexivity].
+
+Ltac2 solve_fresh () := vm_compute; reflexivity.
+
+Ltac2 step_elab () :=
   lazy_match! goal with
-  | [|- le_term ?l _ _ _ _] => l
-  | [|- le_sort ?l _ _ _] => l
-  | [|- wf_term ?l _ _ _] => l
-  | [|- wf_sort ?l _ _] => l
-  | [|- wf_rule ?l _] => l
-  | [|- wf_ctx ?l _] => l
+  | [|- elab_lang nil _] => constructor
+  | [|- elab_lang _ _] => Control.plus (fun () => apply elab_pf) (fun _ => constructor)
+  | [|- elab_rule _ _ _] => constructor
+  | [|- elab_ctx _ _ _] => constructor
+  | [|- elab_args _ _ _ _ _ [::]] => apply elab_args_nil
+  | [|- elab_args _ _ _ (?n::_) _ ((?n,?t)::_)] =>
+      apply elab_args_cons_ex
+  | [|- elab_args _ _ _ _ _ ((?n,?t)::_)] =>
+      eapply elab_args_cons_im
+  (* special case to force existentials to the empty list*)
+  | [|- elab_subst _ _ _ (Core.with_names_from [::] ?l) [::]] =>
+        assert ($l = [::]) > [reflexivity | apply elab_subst_nil]
+  | [|- elab_subst _ _ _ _ [::]] => apply elab_subst_nil
+  | [|- elab_subst _ _ ((?n,?e)::_) ((?n,?ee)::_) ((?n,?t)::_)] =>
+      apply elab_subst_cons_ex > [solve_fresh ()| | |]
+  | [|- elab_subst _ _ _ ((?n,?ee)::_) ((?n,?t)::_)] =>
+      eapply elab_subst_cons_im > [solve_fresh ()| | |]
+  | [|- Core.le_args _ _ _ _ _] =>constructor
+  | [|- Core.wf_args _ _ _ _] =>first [apply wf_args_no_conv_recognizes; vm_compute; reflexivity
+                                     | apply Core.wf_sort_by']
+  | [|- Core.wf_subst _ _ _ _] =>constructor
+  | [|- elab_sort _ _ _ _] => apply elab_sort_by'
+  | [|- Core.wf_sort _ _ _] => first [apply wf_sort_no_conv_recognizes; vm_compute; reflexivity
+                                     | apply Core.wf_sort_by']
+  | [|- Core.wf_term _ _ (Exp.var _) _] => apply Core.wf_term_var
+  | [|- Core.wf_term _ _ _ _] => try (apply wf_term_no_conv_recognizes; vm_compute; reflexivity)
+  | [|- elab_term _ _ (var _) _ _] => apply elab_term_var; solve_in()
+  | [|- elab_term _ _ _ (Exp.var _) _] => apply elab_term_var; solve_in()
+  | [|- is_true((?n,?e)\in ?l)]=> 
+      assert ($e = named_list_lookup $e $l $n); vm_compute; solve[auto]
+  | [|- is_true (_ \in _)] => solve_in ()
+  | [|- is_true (fresh _ _)] => solve_fresh ()
+  | [|- is_true (_ \notin _)] => solve_fresh ()
+  | [|- is_true (subseq _ _)] => vm_compute; reflexivity
+  | [|- is_true true] => reflexivity
+  | [|- len_eq _ _] => constructor  
+  | [|- _ = _] => try (solve[reflexivity| cbv; f_equal])          
 end.
 
-
-
-
-Ltac2 unify_eq () :=
-  match! goal with
-    [|- ?a = ?b] =>
-    solve[f_equal; eauto]
+(* TODO: move to tactics or utils*)
+Require Import Ltac2.Constr.
+Ltac2 is_evar e :=
+  match Unsafe.kind e with
+  | Unsafe.Evar _ _ => true
+  | _ => false
   end.
 
-(* TODO: generalize over key, value types? *)
-Ltac2 Type rec FinMap :=
-  [ MapEmpty
-  | MapCons (constr (*Coq string*), constr, FinMap)].
+Ltac2 shelve_if b :=
+  match b with
+  | true => Control.shelve ()
+  | false => ()
+  end.
 
-Ltac2 Type exn ::= [EmptyMapLookupExn].
-Ltac2 rec map_lookup n m :=
-  match m with
-  | MapEmpty => Control.zero EmptyMapLookupExn
-  | MapCons n' v m' =>
-    match Constr.equal n' n with
-    | true => v
-    | false => map_lookup n m'
-    end
+Ltac2 error_if b e :=
+  match b with
+  | true => Control.zero e
+  | false => ()
   end.
 
 
-
-(* Computes a map that has all mappings from both,
-   or throws if none exists
-TODO: optimize representation for this operation
- *)
-Ltac2 Type exn ::= [MapMergeExn(constr, constr)].
-Ltac2 rec map_merge m1 m2 :=
-  match m1 with
-  | MapEmpty => m2
-  | MapCons k v1 m1' =>
-    MapCons k v1
-            (Control.plus
-               (fun _ => let v2 := map_lookup k m2 in
-                match Constr.equal v1 v2 with
-                | true => map_merge m1' m2
-                | false => Control.zero (MapMergeExn v1 v2)
-                end)
-               (fun ex =>
-                  match ex with
-                  | EmptyMapLookupExn => map_merge m1' m2
-                  | _ => Control.zero ex
-                  end))
-  end.
-
-Ltac2 Type exn ::= [DomainExn(constr, constr, constr)].
-Ltac2 dom_exn c t := DomainExn c (Constr.type c) t.
-
-Ltac2 Type exn ::= [ExpMatchExn(constr, constr)].
-Ltac2 rec exp_match (p : constr) e :=
-  lazy_match! p with
-  | var ?x => MapCons x e MapEmpty
-  | con ?pn ?ps =>
-    (* TODO: handle when e is an existential *)
-    lazy_match! e with
-    | con ?n ?s =>
-      match Constr.equal pn n with
-      | true => exp_list_match ps s
-      | false => Control.throw (ExpMatchExn p e)
-      end
-    | var _ => Control.throw (ExpMatchExn p e)
-    | _ => Control.throw (dom_exn e constr:(exp))
-      (* TODO: need to handle evars*)
-    end
-  | _ => Control.throw (dom_exn p constr:(exp))
-  end
-with exp_list_match p s :=
-    lazy_match! p with
-    | [::] => lazy_match! s with [::] => MapEmpty end
-    | ?pe::?p' =>
-      lazy_match! s with
-      | ?e::?s' =>
-        map_merge (exp_match pe e) (exp_list_match p' s')
-      | [::] => Control.throw (ExpMatchExn p s)
-      end
-end.
-
-Ltac2 sort_match p e :=
-  lazy_match! p with
-  | srt ?pn ?ps =>
-    (* TODO: handle when e is an existential *)
-    lazy_match! e with
-    | srt ?n ?s =>
-      match Constr.equal pn n with
-      | true => exp_list_match ps s
-      | false => Control.throw (ExpMatchExn p e)
-      end
-    | var _ => Control.throw (ExpMatchExn p e)
-    | _ => Control.throw (dom_exn e constr:(exp))
-      (* TODO: need to handle evars*)
-    end
-  | _ => Control.throw (dom_exn p constr:(exp))
-  end.
-  
-
-(* Convert a map into a substition constr
-   according to its output ctx constr *)
-Ltac2 rec subst_of_map m c :=
-  lazy_match! c with
-  | [::] => constr:([::])
-  | (?n,_)::?c' =>
-    let v := map_lookup n m in
-    let tl := subst_of_map m c' in
-    constr:(($n,$v)::$tl)
-  end.
-
-Ltac2 Type exn ::= [JudgmentMismatchExn(constr, constr)].
-Ltac2 apply_rule (name : constr) :=
-  let l := goal_lang () in
-  (* TODO: make d an evar so it isn't silently returned?*)
-  let d := constr:(sort_rule [::]) in
-  let r := Std.eval_cbv all_red_flags
-           constr:(named_list_lookup $d $l $name) in
-  lazy_match! r with
-  | sort_rule ?c' =>
-    lazy_match! goal with
-    | [|- wf_sort ?l ?c ?t] =>
-      eapply (@wf_sort_by $l $c $name) >
-      [ unify_in ()|]
-    | [|- ?j] =>
-      Control.zero
-        (JudgmentMismatchExn constr:(($name,$r)) j)
-    end
-  | term_rule ?c' ?t' =>
-    lazy_match! goal with
-    | [|- wf_term ?l ?c ?e ?t] =>
-      ltac1:(l c e t t'|-
-             let s := fresh "s" in
-             evar (s : subst);
-             replace (wf_term l c e t) with
-                (wf_term l c e t'[/s/]);
-            unfold s;
-            clear s
-            ) (Ltac1.of_constr l)
-              (Ltac1.of_constr c)
-              (Ltac1.of_constr e)
-              (Ltac1.of_constr t)
-              (Ltac1.of_constr t') >
-            [ eapply (@wf_term_by $l $c $name) >
-              [ unify_in () |]
-            | unify_eq()]
-    | [|- ?j] =>
-      Control.zero
-        (JudgmentMismatchExn constr:(($name,$r)) j)
-    end
-  | sort_le ?c' ?t1' ?t2' =>
-    lazy_match! goal with
-    | [|- le_sort ?l ?c ?t1 ?t2] =>
-      let m := map_merge
-                 (sort_match t1' t1)
-                 (sort_match t2' t2) in
-      let s := subst_of_map m c' in
-      my_change2
-        '(le_sort $l $c $t1 $t2)
-        '(le_sort $l $c $t1'[/$s/] $t2'[/$s/]);
-      eapply le_sort_subst;
-      Control.enter
-        (fun () =>
-           match! goal with
-           | [|- le_sort _ _ _ _] =>
-             eapply le_sort_by;
-             unify_in ()
-           | [|- le_subst _ _ _ _ _] => ()
-           | [|- _] => Control.throw Match_failure
-           end)
-    | [|- ?j] =>
-      Control.zero
-        (JudgmentMismatchExn constr:(($name,$r)) j)
-    end
-      
-end.
-(* TODO:
-Check wf_sort_by.
-Goal le_sort [:: [s> |-("req") #"foo" = #"bar"]] [::] (srt "foo" [::])
-(srt "bar" [::]).
-Proof.
-  
-  apply_rule constr:("req"%string).
-  
-  admit.
-  cbv.
-  unfold substable_sort.
-  f_equal; eauto.
-  unify_eq ().
-  
-TODO: deconstruct subst automatically based on c'  
-
-
-
-Ltac2 Eval (exp_match constr:(var 1) constr:(var 2)).
-Ltac2 Eval
-      (exp_match constr:(con 1 [:: var 2; var 2])
-                          constr:(con 1 [:: (con 2 [::]); (con 2 [::])])).
-
-
-(* assumes idx <= size 
-   TODO: how to handle terms that aren't listed?
-   evar?
+(*_TODO: check if necessary anymore
+Transparent get_rule_args.
+Transparent get_rule_ctx.
 *)
-Ltac2 subst_of_map m size :=
-  let rec som idx acc :=
-      match Int.equal idx size with
-      | true => acc
-      | false =>
-        let v := map_lookup idx m in
-        som (Int.add idx 1) constr:($v::$acc)
-      end in
-  som 0 constr:(@nil exp).
 
-Ltac2 Eval (subst_of_map
-              (MapCons 2 constr:(var 3)
-              (MapCons 0 constr:(var 1)
-              (MapCons 1 constr:(var 2) MapEmpty)))) 3.
+Ltac2 elab_term_by ():=
+    apply elab_term_by'; repeat(simpl;step_elab()).
 
-Ltac2 max n m :=
-  match Int.gt n m with
-  | true => n
-  | false => m
+
+Require Import Ltac2.Constr.
+Ltac2 refine_elab pat :=
+  let g := match! goal with
+           | [|- elab_term _ _ _ ?g _] => g
+           | [|- elab_sort _ _ _ ?g ] => g
+           | [|- Core.wf_term _ _ ?g _] => g
+           | [|- Core.wf_sort _ _ ?g] => g
+           end in
+  match Unsafe.kind g with
+  | Unsafe.Evar n _ => Control.new_goal n > [| refine pat]
+  | _ => ()
   end.
 
-Ltac2 rec min_subst_size m :=
-  match m with
-  | MapEmpty => 0
-  | MapCons n _ m' =>
-    max (Int.add n 1) (min_subst_size m')
+Ltac2 inst_elab pat :=
+  let g := match! goal with
+           | [|- elab_term _ _ ?g _ _] => g
+           | [|- elab_sort _ _ ?g _ ] => g
+           | [|- Core.wf_term _ ?g _ _] => g
+           | [|- Core.wf_sort _ ?g _] => g
+           end in
+  match Unsafe.kind g with
+  | Unsafe.Evar n _ => Control.new_goal n > [| refine pat]
+  | _ => ()
   end.
-
-Require Import Ltac2.Notations.
-
-Ltac2 rec unify_in () :=
-  match! goal with
-    [|- is_true (?r \in ?r'::?l)] =>
-    rewrite in_cons;
-    ltac1:(apply /orP);
-    Control.plus
-      (fun () => left;ltac1:(apply /eqP; by f_equal))
-      (fun _ =>
-         right; unify_in ())
-end.
-
-Ltac2 apply_term_rule n :=
-  match! goal with
-    [|- le_term ?l ?c ?t ?e1 ?e2 ]=>
-    match! Std.eval_hnf constr:(nth_level (sort_rule [::]) $l $n) with
-      term_le _ ?pe1 ?pe2 ?pt =>
-      let m := subst_match constr:([:: $pt; $pe1; $pe2])
-                           constr:([:: $t; $e1; $e2]) in
-      let s := subst_of_map m (min_subst_size m) in
-      my_change2
-        constr:(le_term $l $c $t $e1 $e2)
-        constr:(le_term $l $c $pt[/$s/] $pe1[/$s/] $pe2[/$s/]);
-      eapply le_term_subst;
-      Control.enter
-        (fun () =>
-           match! goal with
-           | [|- le_term _ _ _ _ _] =>
-             eapply le_term_by;
-             unify_in ()
-           | [|- le_subst _ _ _ _ _] => ()
-           | [|- _] => Control.throw Match_failure
-           end)
-    end
-end.
-
-
-*)
